Pdl/Fresh.lean
@@ -1,0 +1,71 @@
+
+import Pdl.Vocab
+
+mutual
+  /-- Get a fresh atomic proposition `x` not occuring in `ψ`. -/
+  def freshVarForm : Formula → Nat
+    | ⊥ => 0
+    | ·c => c + 1
+    | ~φ => freshVarForm φ
+    | φ1⋀φ2 => max (freshVarForm φ1) (freshVarForm φ2)
+    | ⌈α⌉ φ => max (freshVarProg α) (freshVarForm φ)
+  /-- Get a fresh atomic proposition `x` not occuring in `α`. -/
+  def freshVarProg : Program → Nat
+    | ·c => c + 1
+    | α;'β  => max (freshVarProg α) (freshVarProg β)
+    | α⋓β  =>  max (freshVarProg α) (freshVarProg β)
+    | ∗α  => freshVarProg α
+    | ?'φ  => freshVarForm φ
+end
+
+open HasVocabulary
+
+mutual
+theorem freshVarForm_is_larger (φ) : ∀ n ∈ voc φ, n < freshVarForm φ := by
+  cases φ
+  all_goals simp [freshVarForm, voc, vocabOfFormula, not_or]
+  case neg φ =>
+    apply freshVarForm_is_larger
+  case and φ1 φ2 =>
+    have IH1 := freshVarForm_is_larger φ1
+    have IH2 := freshVarForm_is_larger φ2
+    aesop
+  case box α φ =>
+    have IHφ := freshVarForm_is_larger φ
+    have IHα := freshVarProg_is_larger α
+    aesop
+
+theorem freshVarProg_is_larger (α) : ∀ n ∈ voc α, n < freshVarProg α := by
+  cases α
+  all_goals simp [freshVarProg, voc, vocabOfProgram]
+  case union α β =>
+    have IHα := freshVarProg_is_larger α
+    have IHβ := freshVarProg_is_larger β
+    aesop
+  case sequence α β =>
+    have IHα := freshVarProg_is_larger α
+    have IHβ := freshVarProg_is_larger β
+    aesop
+  case star α =>
+    have IHα := freshVarProg_is_larger α
+    aesop
+  case test φ =>
+    have IHφ := freshVarForm_is_larger φ
+    aesop
+end
+
+theorem freshVarForm_is_fresh (φ) : freshVarForm φ ∉ voc φ := by
+  have := freshVarForm_is_larger φ
+  simp [freshVarForm, voc, vocabOfFormula] at *
+  by_contra hyp
+  specialize this (freshVarForm φ)
+  have := Nat.lt_irrefl (freshVarForm φ)
+  tauto
+
+theorem freshVarProg_is_fresh (α) : freshVarProg α ∉ HasVocabulary.voc α := by
+  have := freshVarProg_is_larger α
+  simp [freshVarProg, voc, vocabOfFormula] at *
+  by_contra hyp
+  specialize this (freshVarProg α)
+  have := Nat.lt_irrefl (freshVarProg α)
+  tauto
